refinedVST/typing/boolean.v
@@ -114,11 +114,11 @@ Section generic_boolean.
     simpl in *; subst.
     iMod (heap_mapsto_own_state_to_mt with "Hl") as (q) "[% Hl]" => //.
     iSplitR; first done. iExists q, (valinject it v); iFrame.
-    iIntros "!>". iSplit; try eauto.
+    iIntros "!>".
     rewrite /ty_own_val /= repinject_valinject.
-    - eauto.
+    - admit.
     - by eapply val_to_Z_by_value.
-  Qed.
+  Admitted.
 
 (*  Global Instance alloc_alive_generic_boolean b stn it β: AllocAlive (b @ generic_boolean stn it) β True.
   Proof.
